configuration and README update

HoareVerification/oldMachine.lean
@@ -1,1 +1,311 @@
-def hello := "world"
+
+/-
+
+A register machine is sequence of instructions of the form
+
+  CLR (r): CLeaR register r. (Set r to zero.)
+  INC (r): INCrement the contents of register r.
+  DEC (r): DECrement the contents of register r.
+  CPY (rj, rk): CoPY the contents of register rj to register rk leaving the contents of rj intact.
+  JZ (r, z): IF register r contains Zero THEN Jump to instruction z ELSE continue in sequence.
+  JE (rj, rk, z): IF the contents of register rj Equals the contents of register rk THEN Jump to instruction z ELSE continue in sequence.
+
+We also add
+
+  SET (r,v) : SET the value of register r to v
+
+In Lean, we can define an inductive type to capture these rules syntactically.
+
+-/
+
+/-
+# TYPES
+-/
+
+namespace RM
+
+structure State where
+  pc : Nat
+  mem : Nat → Nat
+
+def init : State := ⟨ 0, λ _ => 0 ⟩
+
+abbrev Action := State → State
+abbrev Program := List Action
+
+/-
+# INSTRUCTIONS
+-/
+
+@[simp]
+def set (r val : Nat) : Action := λ s => ⟨
+  s.pc+1,
+  λ x => if x = r then val else s.mem x
+⟩
+
+@[simp]
+def dec (r : Nat) : Action := λ s => ⟨
+  s.pc+1,
+  λ x => if x = r then s.mem x - 1 else s.mem x
+⟩
+
+@[simp]
+def jz (r loc : Nat) : Action := λ s =>  ⟨
+  if s.mem r = 0 then loc else s.pc+1,
+  s.mem
+⟩
+
+@[simp]
+abbrev goto loc := jz 0 loc
+
+@[simp]
+def inc (r : Nat) : Action := λ s => ⟨
+  s.pc+1,
+  λ x => if x = r then s.mem x + 1 else s.mem x
+⟩
+
+@[simp]
+def clr (r : Nat) : Action := λ s => ⟨
+  s.pc+1,
+  λ x => if x = r then 0 else s.mem x
+⟩
+
+@[simp]
+def cpy (rj rk : Nat) : Action := λ s => ⟨
+  s.pc+1,
+  λ x => if x = rk then s.mem rj else s.mem x
+⟩
+
+@[simp]
+def je (rj rk z: Nat) : Action := λ s => ⟨
+  if s.mem rj = s.mem rk then z else s.pc + 1,
+  s.mem
+⟩
+
+
+/-
+# PROGRAMS
+-/
+
+def step (p : Program) : Action := λ s =>
+  if h : s.pc < p.length
+  then p[s.pc] s
+  else s
+
+def run (p : Program) (numsteps : Nat) : Action := λ s =>
+  match numsteps with
+  | Nat.zero => s
+  | Nat.succ k => run p k (step p s)
+
+/-
+# EXAMPLE
+-/
+
+def P1 : Program := [
+  set 1 10,
+  dec 1,
+  jz 1 4,
+  goto 1
+]
+
+
+
+/-
+
+0
+2
+3
+0
+0
+
+One way to do it:
+0. Initialize r1 and r2
+1. incr r3 and r4 until r3 equals r2.
+2. Set r3 to zero and decr r1
+3. Repeat steps 1 and 2 until r1 = 0.
+
+
+This wants to be a while loop!
+-/
+
+
+def set_mul : Program := [
+  -- Set initial values
+  set 1 5,
+  set 2 5,
+  -- incr r3 and r4
+  inc 3,
+  inc 4,
+  -- Check to see if r3 = r2. If so, reset, if not, inc again
+  je 2 3 6,
+  goto 2,
+  -- reset
+  dec 1,
+  set 3 0,
+  -- Check if we're done, if not, loop.
+  jz 1 10,
+  goto 2
+]
+
+#eval (run set_mul 1000 init ).mem 4
+
+-- Multiply values at r1 and r2 and store value at r4.
+-- Starting assumptions:
+def mul : Program := [
+  inc 3,
+  inc 4,
+  je 2 3 4,
+  goto 0,
+  dec 1,
+  set 3 0,
+  jz 1 10,
+  goto 0
+]
+
+
+/-Idea: write something that compiles a program from higher level language into a program. -/
+
+#eval (run set_mul 54 init ).mem 4
+
+def s1 := set 1 5 init
+def s2 := set 2 5 s1
+
+#eval (run mul 1000 s2).mem 4
+
+/-
+# HOARE LOGIC
+-/
+
+def Hoare (P : State → Prop)
+          (T : State → State)
+          (Q : State → Prop) :=
+  ∀ s, P s → Q (T s)
+
+def comp (T₁ T₂ : State → State) := (λ s => T₂ (T₁ s))
+
+theorem hoare_compose {P R: State → Prop} {T₁ T₂ : State → State}
+  : (∃ Q , Hoare P T₁ Q ∧ Hoare Q T₂ R) → Hoare P (comp T₁ T₂) R := by
+    intro ⟨ Q, ⟨ hpq, hqr ⟩ ⟩ s hs
+    exact hqr (T₁ s) (hpq s hs)
+
+theorem hoare_consequence
+  {P₁ P₂ Q₁ Q₂: State → Prop} {T : State → State}
+  {hp : ∀ s, P₁ s → P₂ s} {hq : ∀ s, Q₂ s → Q₁ s}
+  : Hoare P₂ T Q₂ → Hoare P₁ T Q₁ := by
+    intro hpq s hs
+    apply hq (T s)
+    apply hpq s
+    apply hp s
+    exact hs
+
+/- CONdition AND: True when both conditions are met-/
+def con_and (P₁ P₂ : State → Prop) := λ s => P₁ s ∧ P₂ s
+
+/-CONdition NOT: -/
+def con_not (P : State → Prop) := λ s => P s → False
+
+def ite (T₁ T₂ : State → State) (B : State → Prop) [DecidablePred B] :=
+  λ s => if B s then T₁ s else T₂ s
+
+theorem hoare_conditional {B P Q: State → Prop} {T₁ T₂ : State → State} [DecidablePred B]
+  : (Hoare (con_and B P) T₁ Q ∧ Hoare (con_and (con_not B) P) T₂ Q) →
+  Hoare P (ite T₁ T₂ B) Q := by
+    unfold Hoare con_and con_not ite
+    intro h s hps
+    by_cases hbs : (B s)
+    . split
+      exact h.left s ⟨ hbs, hps ⟩
+      contradiction
+    . split
+      . contradiction
+      . exact h.right s ⟨ hbs, hps ⟩
+
+
+
+/-
+# HOARE LOGIC EXAMPLES
+-/
+
+example : Hoare (λ s => s.pc = 0)
+                (run P1 1)
+                (λ s => s.pc = 1) := by
+  intro s hs
+  simp[run,step,P1]
+  rw[hs]
+  simp[hs]
+
+example : Hoare (λ s => s.mem 1 = 0)
+                (comp (set 1 10) (dec 1))
+                (λ s => s.mem 1 = 9) := by
+  apply hoare_compose
+  apply Exists.intro λ s => s.mem 1 = 10
+  simp[Hoare]
+  intro s hs
+  simp[hs]
+
+/- It seems harder to reason about `run` possibly becuase you have
+   to keep track of the program counter. -/
+example : Hoare (λ s => s.pc = 0 ∧ s.mem 1 = 0)
+                (run P1 2)
+                (λ s => s.pc = 2 ∧ s.mem 1 = 9) := by
+  apply hoare_compose
+  apply Exists.intro λ s => s.pc = 1 ∧ s.mem 1 = 10
+  apply And.intro
+  . intro s ⟨ hp, hm ⟩
+    simp[P1,step]
+    rw[hp]
+    simp[hp]
+  . intro s ⟨ hp, hm ⟩
+    simp[P1,run,step]
+    rw[hp]
+    simp[hp]
+    simp_all
+
+
+
+
+
+
+
+
+/-
+# THEOREMS ABOUT INSTRUCTIONS
+-/
+theorem jz_effect {i j k: Nat}
+  : Hoare (λ s => s.pc = i ∧ s.mem j = 0)
+          (jz j k)
+          (λ s => s.pc = k) := by
+  intro s ⟨ hpc, hmem ⟩
+  simp[run,step,P1,hpc,hmem]
+
+theorem set_effect {r u v: Nat}
+  : Hoare (λ s => s.mem r = u)
+          (set r v)
+          (λ s => s.mem r = v) := by
+  intro s h
+  simp[run,step,P1,h]
+
+
+
+
+  /-
+  Two notions of programs:
+  1. List of instructions
+  2. If then else produces a program instead of an action
+  3. Theorems on the program level
+  4. Relocatable code
+
+  Rewrite compose using concatination of programs
+  Rewrite if then else using something like concatination
+  Prove mult using only Hoare triples that work on lists
+
+  1. Problems: Datatypes
+  2. Relate to bytecode
+
+  Risc 5 with Hoare triples
+
+
+  MD book on machine thing
+
+  clone repo of Eric's book
+  -/
