HoareVerification/machine.lean
@@ -1,0 +1,16 @@
+/-
+
+A register machine is sequence of instructions of the form
+
+  CLR (r): CLeaR register r. (Set r to zero.)
+  INC (r): INCrement the contents of register r.
+  DEC (r): DECrement the contents of register r.
+  CPY (rj, rk): CoPY the contents of register rj to register rk leaving the contents of rj intact.
+  JZ (r, z): IF register r contains Zero THEN Jump to instruction z ELSE continue in sequence.
+  JE (rj, rk, z): IF the contents of register rj Equals the contents of register rk THEN Jump to instruction z ELSE continue in sequence.
+
+We also add
+
+  SET (r,v) : SET the value of register r to v
+
+--/
