Main.lean
@@ -1,4 +1,3 @@
-import HoareVerification
 
 def main : IO Unit :=
-  IO.println s!"Hello, {hello}!"
+  IO.println "Hello, Lean"
